@prefix : <http://purl.org/aiaontology/gsvocabulary#> .
@prefix aia: <http://purl.org/aiaontology#> .
@prefix owl: <http://www.w3.org/2002/07/owl#> .
@prefix rdf: <http://www.w3.org/1999/02/22-rdf-syntax-ns#> .
@prefix xml: <http://www.w3.org/XML/1998/namespace> .
@prefix xsd: <http://www.w3.org/2001/XMLSchema#> .
@prefix cdmv: <http://purl.org/aiaontology/cdmvocabulary#> .
@prefix rdfs: <http://www.w3.org/2000/01/rdf-schema#> .
@prefix skos: <http://www.w3.org/2004/02/skos/core#> .
@prefix vcsv: <http://purl.org/aiaontology/vcsvocabulary#> .
@base <http://purl.org/aiaontology/gsvocabulary> .

<http://purl.org/aiaontology/gsvocabulary> rdf:type owl:Ontology ;
                                            owl:imports <http://purl.org/aiaontology> ;
                                            <http://purl.org/dc/terms/description> "This vocabulary integrates common glossary terms related to Gold Standard-compliant climate action projects with the aia ontology for (general) anthropogenic impact accounting. You can find more about the aia-o <a href=\"https://wiki.hyperledger.org/display/CASIG/An+ontology+for+anthropogenic+impact+accounting\">here</a>."@en ;
                                            <http://purl.org/dc/terms/source> <https://globalgoals.goldstandard.org/faqs-glossary/#> ;
                                            <http://purl.org/dc/terms/title> "Gold Standard Vocabulary"@en ;
                                            rdfs:comment "Terms and their definitions are drawn directly from the GS glossary at this source unless indicated otherwise. Definitions from this glossary are indicated by skos:definition; from other sources by rdfs:comment"@en .

#################################################################
#    Annotation properties
#################################################################

###  http://www.w3.org/2002/07/owl#equivalentClass
owl:equivalentClass rdf:type owl:AnnotationProperty .


###  http://www.w3.org/2002/07/owl#equivalentProperty
owl:equivalentProperty rdf:type owl:AnnotationProperty .


###  http://www.w3.org/2002/07/owl#sameAs
owl:sameAs rdf:type owl:AnnotationProperty .


###  http://www.w3.org/2004/02/skos/core#altLabel
skos:altLabel rdf:type owl:AnnotationProperty .


###  http://www.w3.org/2004/02/skos/core#definition
skos:definition rdf:type owl:AnnotationProperty .


###  http://www.w3.org/2004/02/skos/core#related
skos:related rdf:type owl:AnnotationProperty .


#################################################################
#    Datatypes
#################################################################

###  http://purl.org/aiaontology/gsvocabulary#Gt
:Gt rdf:type rdfs:Datatype ;
    rdfs:comment "Giga-Tonne"@en .


###  http://purl.org/aiaontology/gsvocabulary#MWel
:MWel rdf:type rdfs:Datatype ;
      rdfs:comment "Mega-Watt Electrical"@en .


###  http://purl.org/aiaontology/gsvocabulary#MWh
:MWh rdf:type rdfs:Datatype ;
     rdfs:comment "Mega-Watt per hour"@en .


###  http://purl.org/aiaontology/gsvocabulary#MWth
:MWth rdf:type rdfs:Datatype ;
      rdfs:comment "Mega-Watt Thermal"@en .


###  http://purl.org/aiaontology/gsvocabulary#TRUE
:TRUE rdf:type rdfs:Datatype .


###  http://purl.org/aiaontology/gsvocabulary#kW
:kW rdf:type rdfs:Datatype ;
    rdfs:comment "Kilo-Watt"@en .


#################################################################
#    Object Properties
#################################################################

###  http://purl.org/aiaontology/gsvocabulary#CPAhasPDD
:CPAhasPDD rdf:type owl:ObjectProperty ;
           rdfs:domain :CDMProgrammeActivity ;
           rdfs:range :ProjectDesignDocument .


###  http://purl.org/aiaontology/gsvocabulary#auditorInTeam
:auditorInTeam rdf:type owl:ObjectProperty ;
               rdfs:domain aia:Auditor ;
               rdfs:range :AuditTeam .


###  http://purl.org/aiaontology/gsvocabulary#disputeWith
:disputeWith rdf:type owl:ObjectProperty ;
             rdfs:domain :AssuranceProvider ;
             rdfs:range aia:Agent .


###  http://purl.org/aiaontology/gsvocabulary#disputesClaim
:disputesClaim rdf:type owl:ObjectProperty ;
               rdfs:domain aia:Claim ;
               rdfs:range aia:Claim .


###  http://purl.org/aiaontology/gsvocabulary#fulfillsRequirement
:fulfillsRequirement rdf:type owl:ObjectProperty ;
                     rdfs:domain owl:Thing ;
                     rdfs:range <http://purl.org/aiaontology#Control(n)> .


###  http://purl.org/aiaontology/gsvocabulary#givenInFeedbackRound
:givenInFeedbackRound rdf:type owl:ObjectProperty ;
                      rdfs:domain :Feedback ;
                      rdfs:range :StakeholderFeedbackRound .


###  http://purl.org/aiaontology/gsvocabulary#givesFeedback
:givesFeedback rdf:type owl:ObjectProperty ;
               rdfs:domain :RelevantStakeholders ;
               rdfs:range :Feedback .


###  http://purl.org/aiaontology/gsvocabulary#hasDesignCertification
:hasDesignCertification rdf:type owl:ObjectProperty ;
                        rdfs:domain aia:Activity ;
                        rdfs:range :DesignCertification .


###  http://purl.org/aiaontology/gsvocabulary#hasPerformanceCertification
:hasPerformanceCertification rdf:type owl:ObjectProperty ;
                             rdfs:domain aia:Activity ;
                             rdfs:range :Certification .


###  http://purl.org/aiaontology/gsvocabulary#hasProjectArea
:hasProjectArea rdf:type owl:ObjectProperty ;
                rdfs:domain aia:Activity ;
                rdfs:range aia:Location .


###  http://purl.org/aiaontology/gsvocabulary#hasProjectBoundary
:hasProjectBoundary rdf:type owl:ObjectProperty ;
                    rdfs:domain :ProjectArea ;
                    rdfs:range :ProjectBoundary .


###  http://purl.org/aiaontology/gsvocabulary#influenceReputation
:influenceReputation rdf:type owl:ObjectProperty ;
                     rdfs:domain :Complaints ;
                     rdfs:range aia:Reputation .


###  http://purl.org/aiaontology/gsvocabulary#usedToSupport
:usedToSupport rdf:type owl:ObjectProperty ;
               rdfs:domain :KeyProjectInformation ;
               rdfs:range :EligibilityCheck .


#################################################################
#    Data properties
#################################################################

###  http://purl.org/aiaontology#hasUnitOfMeasure
aia:hasUnitOfMeasure rdf:type owl:DatatypeProperty .


###  http://purl.org/aiaontology/gsvocabulary#equivalentTo
:equivalentTo rdf:type owl:DatatypeProperty ;
              rdfs:comment "Used to indicate aggregated or equivalent units of measurement."@en .


###  http://purl.org/aiaontology/gsvocabulary#hasImplementationDate
:hasImplementationDate rdf:type owl:DatatypeProperty ;
                       rdfs:domain aia:Activity ;
                       rdfs:range xsd:dateTime .


###  http://purl.org/aiaontology/gsvocabulary#isCompotent
:isCompotent rdf:type owl:DatatypeProperty ;
             rdfs:domain aia:Agent ;
             rdfs:range xsd:boolean ;
             rdfs:comment "FIX: possibly use reification to make a statement (a Claim) about this statement"@en .


#################################################################
#    Classes
#################################################################

###  http://purl.org/aiaontology#Activity
aia:Activity rdf:type owl:Class .


###  http://purl.org/aiaontology#Agent
aia:Agent rdf:type owl:Class .


###  http://purl.org/aiaontology#Auditor
aia:Auditor rdf:type owl:Class ;
            owl:equivalentClass [ rdf:type owl:Restriction ;
                                  owl:onProperty :isCompotent ;
                                  owl:allValuesFrom xsd:boolean
                                ] ;
            rdfs:subClassOf aia:Role ;
            rdfs:comment "FIX condition so that the value for isCompotent can be only TRUE"@en ,
                         "Person who carries out the audit"@en .


###  http://purl.org/aiaontology#Claim
aia:Claim rdf:type owl:Class ;
          rdfs:subClassOf <http://purl.org/aiaontology#Audit(n)> .


###  http://purl.org/aiaontology#Control
aia:Control rdf:type owl:Class .


###  http://purl.org/aiaontology#Indicator
aia:Indicator rdf:type owl:Class .


###  http://purl.org/aiaontology#LegalPerson
aia:LegalPerson rdf:type owl:Class ;
                rdfs:subClassOf aia:Agent .


###  http://purl.org/aiaontology#Location
aia:Location rdf:type owl:Class .


###  http://purl.org/aiaontology#Objective
aia:Objective rdf:type owl:Class .


###  http://purl.org/aiaontology#Output
aia:Output rdf:type owl:Class .


###  http://purl.org/aiaontology#Parameter
aia:Parameter rdf:type owl:Class .


###  http://purl.org/aiaontology#Period
aia:Period rdf:type owl:Class .


###  http://purl.org/aiaontology#Procedure
aia:Procedure rdf:type owl:Class .


###  http://purl.org/aiaontology#Process
aia:Process rdf:type owl:Class .


###  http://purl.org/aiaontology#Report
aia:Report rdf:type owl:Class .


###  http://purl.org/aiaontology#Reputation
aia:Reputation rdf:type owl:Class .


###  http://purl.org/aiaontology#Resource
aia:Resource rdf:type owl:Class .


###  http://purl.org/aiaontology#Role
aia:Role rdf:type owl:Class .


###  http://purl.org/aiaontology#State
aia:State rdf:type owl:Class .


###  http://purl.org/aiaontology#Audit(n)
<http://purl.org/aiaontology#Audit(n)> rdf:type owl:Class ;
                                       rdfs:subClassOf <http://purl.org/aiaontology#Claim(n)> .


###  http://purl.org/aiaontology#Claim(n)
<http://purl.org/aiaontology#Claim(n)> rdf:type owl:Class .


###  http://purl.org/aiaontology#Control(n)
<http://purl.org/aiaontology#Control(n)> rdf:type owl:Class ;
                                         owl:equivalentClass :Requirements .


###  http://purl.org/aiaontology/gsvocabulary#AffectedStakeholder
:AffectedStakeholder rdf:type owl:Class ;
                     rdfs:subClassOf :RelevantStakeholders ;
                     skos:definition "Any stakeholder affected physically, socially or economically by the implementation of the Project. Note that affected stakeholders may be outside the Project Area and in some cases be a distance beyond the Project Boundary."@en .


###  http://purl.org/aiaontology/gsvocabulary#AnnualReport
:AnnualReport rdf:type owl:Class ;
              rdfs:subClassOf aia:Report ;
              rdfs:comment "An annual update submitted by the Project Developer. Report covers updates and actions taken on the Project during a given year."@en ,
                           "FIX: depending on updates to aia, this may need to be a subclass of Claim instead"@en .


###  http://purl.org/aiaontology/gsvocabulary#Assessment
:Assessment rdf:type owl:Class ;
            rdfs:subClassOf aia:Activity ;
            rdfs:comment "TODO: correct taxonomy for activity > verify > audit"@en ;
            skos:definition "The combined process of audit, review and decision on a conformity within the requirements of a standard (part of Validation or Verification e.g. a Validation Assessment)."@en .


###  http://purl.org/aiaontology/gsvocabulary#Assurance
:Assurance rdf:type owl:Class ;
           rdfs:subClassOf <http://purl.org/aiaontology#Control(n)> ;
           rdfs:comment "Demonstrable evidence that specified requirements related to an activity are fulfilled."@en ;
           skos:related vcsv:Proof .


###  http://purl.org/aiaontology/gsvocabulary#AssuranceProvider
:AssuranceProvider rdf:type owl:Class ;
                   rdfs:subClassOf aia:Role .


###  http://purl.org/aiaontology/gsvocabulary#AuditTeam
:AuditTeam rdf:type owl:Class ;
           rdfs:subClassOf aia:Agent ;
           skos:definition "One or more auditors conducting an assessment. An audit team may consist of only one person; in such cases, the person is expected to have all team competences and team leader competences."@en .


###  http://purl.org/aiaontology/gsvocabulary#BaselineScenario
:BaselineScenario rdf:type owl:Class ;
                  rdfs:subClassOf aia:State ;
                  rdfs:comment "The Baseline Scenario is defined as the reasonable, conservative scenario that would exist in the absence of the project. While setting the Baseline Scenario the Project Developer shall take into account the relevant applicable legislation and how effectively these are enforced."@en .


###  http://purl.org/aiaontology/gsvocabulary#CDMProgrammeActivity
:CDMProgrammeActivity rdf:type owl:Class ;
                      rdfs:subClassOf aia:Activity ;
                      rdfs:label "CDM Programme Activity"@en ;
                      skos:altLabel "CPA"@en ;
                      skos:definition "A CDM project activity under a programme of activities. A CPA is a single, or a set of interrelated measure(s), to reduce GHG emissions or result in net anthropogenic greenhouse gas removals by sinks, applied within a designated area defined in the baseline methodology."@en .


###  http://purl.org/aiaontology/gsvocabulary#Certification
:Certification rdf:type owl:Class ;
               rdfs:subClassOf <http://purl.org/aiaontology#Control(n)> ;
               rdfs:comment "TODO: certification is the control we use for fulfillsRequirement"@en ,
                            "The written assurance confirmation/communication that fulfilment of specified requirements has been demonstrated (Adapted from ISO 17000)."@en .


###  http://purl.org/aiaontology/gsvocabulary#CertifiedEmissionsReduction
:CertifiedEmissionsReduction rdf:type owl:Class ;
                             rdfs:subClassOf aia:Claim ;
                             rdfs:comment "A carbon credit is a specific aia:Claim, namely, the claim to be responsible for the environmental benefit equal to one carbon credit."@en ,
                                          "Certified Emissions Reduction: a carbon credit, issued by another third party standard (typically UNFCCC CDM) for use in the compliance carbon markets.  A Gold Standard labelled CER is known as a GS-CER."@en ;
                             skos:altLabel "CER"@en ,
                                           "GS-CER"@en .


###  http://purl.org/aiaontology/gsvocabulary#CleanDevelopmentMechanism
:CleanDevelopmentMechanism rdf:type owl:Class ;
                           rdfs:subClassOf aia:Control ;
                           rdfs:comment "Standard for the issues of Certified Emission Reductions, operated by the UNFCCC."@en ;
                           rdfs:label "Clean Development Mechanism"@en ;
                           skos:altLabel "CDM"@en .


###  http://purl.org/aiaontology/gsvocabulary#CommunityServiceActivity
:CommunityServiceActivity rdf:type owl:Class ;
                          rdfs:subClassOf aia:Activity ;
                          rdfs:label "Community Service Activity"@en ;
                          skos:definition "A Project type that entails provision of services to a community.  The Requirements for CSA are included in the Gold Standard Community Services Activity Requirements."@en .


###  http://purl.org/aiaontology/gsvocabulary#Complaints
:Complaints rdf:type owl:Class ;
            rdfs:subClassOf aia:Claim ;
            rdfs:comment "Formal (written) and/or informal (verbal) expressions of dissatisfaction regarding the performance of an assurance provider in relation to its Gold Standard function(s), from any source, such as the client, the general public or its representatives, government bodies, NGOs, etc."@en .


###  http://purl.org/aiaontology/gsvocabulary#Conformity
:Conformity rdf:type owl:Class ;
            rdfs:subClassOf aia:Activity ;
            owl:disjointWith :NonConformity ;
            skos:definition "Conformity is defined as the fulfillment of a requirement."@en .


###  http://purl.org/aiaontology/gsvocabulary#ConformityCriteria
:ConformityCriteria rdf:type owl:Class ;
                    rdfs:subClassOf <http://purl.org/aiaontology#Control(n)> ;
                    rdfs:comment "A checklist and associated guidance for GS-VVBs for the Validation or Verification against Gold Standard for the Global Goals."@en .


###  http://purl.org/aiaontology/gsvocabulary#CoordinatingAndManagingEntity
:CoordinatingAndManagingEntity rdf:type owl:Class ;
                               rdfs:subClassOf aia:Agent ;
                               rdfs:comment "FIX: isCMEOf & hasCME"@en ;
                               rdfs:label "Coordinating and Managing Entity"@en ;
                               rdfs:seeAlso "Entity that communicates with the Gold Standard on all matters related to a Programme of Activities and associated activities, as nominated in the cover letters to be submitted for each one of the activities."@en .


###  http://purl.org/aiaontology/gsvocabulary#CorrectiveActionRequest
:CorrectiveActionRequest rdf:type owl:Class ;
                         rdfs:subClassOf <http://purl.org/aiaontology#Control(n)> ;
                         rdfs:comment "With a CAR, the GS-VVB (Validation and Verification Body) or The Gold Standard requests appropriate action be taken to show conformity with a requirement. In order to achieve a successful certification, all CARs shall be formally closed."@en ;
                         rdfs:label "Corrective Action Request"@en ;
                         skos:altLabel "CAR"@en .


###  http://purl.org/aiaontology/gsvocabulary#CustomaryRights
:CustomaryRights rdf:type owl:Class ;
                 rdfs:subClassOf aia:Control ;
                 rdfs:comment "Customary rights are those that result from a long series of habitual or customary actions, constantly repeated, which have, by such repetition and by uninterrupted acquiescence, acquired the force of a law within a geographical or sociological unit."@en .


###  http://purl.org/aiaontology/gsvocabulary#DesignCertification
:DesignCertification rdf:type owl:Class ;
                     rdfs:subClassOf aia:Control ;
                     rdfs:comment "Project Design Certification is a key milestone in the Project Cycle. It marks the point a Project has undertaken Validation, a Validation and Verification Body has submitted a positive opinion and the Gold Standard Project Design Review is complete. Only Certified Project Design status Projects may proceed to Verification/Performance Certification (see also Retro-active Registration/merging Project Design Certification and Performance Certification)."@en .


###  http://purl.org/aiaontology/gsvocabulary#DesignatedNationalAuthority
:DesignatedNationalAuthority rdf:type owl:Class ;
                             rdfs:subClassOf aia:LegalPerson ;
                             rdfs:label "Designated National Authority"@en ;
                             skos:altLabel "DNA"@en ;
                             skos:definition "A designated national authority (DNA) is the organization granted responsibility by a Party to authorise and approve participation in CDM projects."@en .


###  http://purl.org/aiaontology/gsvocabulary#DesignatedOperationalEntity
:DesignatedOperationalEntity rdf:type owl:Class ;
                             rdfs:subClassOf :ValidationAndVerificationBody ;
                             rdfs:comment "A type of VVB that is eligible to apply for GS-VVB status.  DOE is the term used by the UNFCCC for VVBs that are accredited to Validate and Verify CDM Projects."@en ;
                             rdfs:label "Designated Operational Entity"@en .


###  http://purl.org/aiaontology/gsvocabulary#Disputes
:Disputes rdf:type owl:Class ;
          rdfs:subClassOf aia:Claim ;
          rdfs:comment "Disagreement between an assurance provider and the client regarding the assurance provider’s recommendation and/or opinions/decisions made at various stages during the audit."@en .


###  http://purl.org/aiaontology/gsvocabulary#EligibilityCheck
:EligibilityCheck rdf:type owl:Class ;
                  rdfs:subClassOf aia:Activity ;
                  rdfs:comment "The activity of checking project eligibility within the Principles & Requirements and the relevant Project Activity Requirements"@en ;
                  rdfs:seeAlso <https://www.goldstandard.org/publications/certification-process-stepbystep> .


###  http://purl.org/aiaontology/gsvocabulary#EligibilityPrinciples
:EligibilityPrinciples rdf:type owl:Class ;
                       rdfs:subClassOf aia:Objective ;
                       rdfs:comment "The overarching rationale and purpose for the Requirements as related to achieving the Gold Standard Vision and Mission."@en .


###  http://purl.org/aiaontology/gsvocabulary#EnvironmentalAndSocialImpactAssessment
:EnvironmentalAndSocialImpactAssessment rdf:type owl:Class ;
                                        rdfs:subClassOf aia:Control ;
                                        rdfs:label "Environmental and Social Impact Assessment"@en ;
                                        skos:altLabel "ESIA"@en .


###  http://purl.org/aiaontology/gsvocabulary#ExpertStakeholder
:ExpertStakeholder rdf:type owl:Class ;
                   rdfs:subClassOf :RelevantStakeholders ;
                   rdfs:comment "TODO: add constraint - an expert stakeholder should have 10+ years of experience etc. per the definition above"@en ;
                   skos:definition "Expert Stakeholders are individuals that hold specific expertise or knowledge about the organization, process, or activity being audited and/or about the context and practices to which the project is applied. For the purposes of this Standard a Stakeholder is considered an expert if they hold over 10 years of relevant, contextually specific professional, academic or practical experience in a given topic. Higher academic qualifications are preferred but can be justified as not required if necessary."@en .


###  http://purl.org/aiaontology/gsvocabulary#Feedback
:Feedback rdf:type owl:Class .


###  http://purl.org/aiaontology/gsvocabulary#ForwardActionRequest
:ForwardActionRequest rdf:type owl:Class ;
                      rdfs:subClassOf <http://purl.org/aiaontology#Control(n)> ;
                      rdfs:comment "Forward Action Request: A Validation & Verification Body (VVB) or The Gold Standard Secretariat requests appropriate action be taken in the project to become fully compliant with a requirement. FARs are not raised for issues that are linked to the eligibility of a project under the WBC scheme, such as a financial needs assessment. A FAR will be issued where the impact of the infraction is: not material within the current certification, AND unusual or non-systematic, AND correctable in a specific timeframe of less than 1 year. FARs can be closed by The Gold Standard Secretariat or a GS-VVB."@en ;
                      rdfs:label "Forward Action Request"@en ;
                      skos:altLabel "FAR"@en .


###  http://purl.org/aiaontology/gsvocabulary#GMO
:GMO rdf:type owl:Class ;
     rdfs:comment "(Source: FSC) An organism in which the genetic material has been altered in a way that does not occur naturally by mating and/or natural recombination. See ‘FSC Interpretation on GMO – FSC-POL-30-602’"@en ;
     rdfs:label "Genetically Modified Organism"@en ;
     rdfs:seeAlso <https://ic.fsc.org/policies.338.htm> .


###  http://purl.org/aiaontology/gsvocabulary#GSMethodology
:GSMethodology rdf:type owl:Class ;
               rdfs:subClassOf aia:Procedure ;
               rdfs:comment "The specific Activity/Outcome requirements and procedures used to calculate, monitor and report on a given Outcome that may lead to the issuance of Gold Standard Certified SDG Impact Statements or Products."@en ;
               rdfs:label "Gold Standard Approved Methodology"@en ;
               skos:related cdmv:approvedMethodology .


###  http://purl.org/aiaontology/gsvocabulary#GSSDGTool
:GSSDGTool rdf:type owl:Class ;
           rdfs:subClassOf aia:Procedure ;
           rdfs:comment "An approved Tool that can be used to demonstrate one or more positive SDG Impacts. They cannot be used for the Issuance of GS Certified SDG Impact Statements or Products."@en ;
           rdfs:label "Gold Standard Approved Sustainable Development Goal Tool"@en ;
           skos:related cdmv:MethodologicalTool .


###  http://purl.org/aiaontology/gsvocabulary#GlobalProtocolForCommunities
:GlobalProtocolForCommunities rdf:type owl:Class ;
                              rdfs:subClassOf aia:Procedure ;
                              rdfs:seeAlso <https://ghgprotocol.org/greenhouse-gas-protocol-accounting-reporting-standard-cities> ;
                              skos:altLabel "GPC"@en .


###  http://purl.org/aiaontology/gsvocabulary#GoldStandardAccreditationApproval
:GoldStandardAccreditationApproval rdf:type owl:Class ;
                                   rdfs:subClassOf aia:Claim ;
                                   rdfs:comment "Formal recognition of a Validation and Verification Body's institutional capacity and competence to be eligible to carry out the GS audit in accordance with the standard requirements."@en .


###  http://purl.org/aiaontology/gsvocabulary#GoldStandardCertifiedProject
:GoldStandardCertifiedProject rdf:type owl:Class ;
                              rdfs:subClassOf :Project ;
                              skos:definition "A Project that has successfully completed Design Certification and completed at least one Performance Certification successfully."@en .


###  http://purl.org/aiaontology/gsvocabulary#GoldStandardCertifiedSDGImpacts
:GoldStandardCertifiedSDGImpacts rdf:type owl:Class ;
                                 rdfs:subClassOf aia:Output ;
                                 rdfs:comment "Gold Standard Certified SDG Impacts are achieved by following GS-Approved Methodologies and successfully undergoing Performance Certification. They may be in the form of Gold Standard Certified Products or SDG Impact Statements, issued upon successful completion of Performance Certification."@en .


###  http://purl.org/aiaontology/gsvocabulary#GoldStandardNGOSupporters
:GoldStandardNGOSupporters rdf:type owl:Class ;
                           rdfs:subClassOf aia:LegalPerson ;
                           rdfs:seeAlso <http://www.goldstandard.org/our-story/who-we-are> ;
                           skos:definition "Gold Standard was founded by a group of NGOs and continues to represent the interests of civil society in all our work. NGO Supporters can take an active role in the project development process, providing constructive feedback and offering their expertise. This lends further credibility to our local sustainable development initiatives. Every NGO that supports Gold Standard helps strengthen the collective statement that carbon markets should foster transparency, environmental rigor and sustainable development."@en .


###  http://purl.org/aiaontology/gsvocabulary#GoldStandardVerifiedEmissionsReduction
:GoldStandardVerifiedEmissionsReduction rdf:type owl:Class ;
                                        rdfs:subClassOf aia:Output ;
                                        rdfs:comment "A Gold Standard issued Verified Emissions Reduction: a single unit (one tonne) of CO2 equivalent reduction captured as a carbon credit for use as a commodity within the voluntary carbon market."@en ;
                                        skos:altLabel "GS-VER"@en .


###  http://purl.org/aiaontology/gsvocabulary#Gold_Standard_Certified_Products
:Gold_Standard_Certified_Products rdf:type owl:Class ;
                                  rdfs:subClassOf :GoldStandardCertifiedSDGImpacts ;
                                  rdfs:comment "Products are a type of Gold Standard Certified SDG Impact that are issued by Gold Standard upon the successful Performance Certification under a given GS Approved Methodology and Product Requirements. Examples include GS VERs and CER Labels."@en .


###  http://purl.org/aiaontology/gsvocabulary#Gold_Standard_Certified_SDG_Impact_Statement
:Gold_Standard_Certified_SDG_Impact_Statement rdf:type owl:Class ;
                                              rdfs:subClassOf :GoldStandardCertifiedSDGImpacts ;
                                              rdfs:comment "A Certified Statement issued by Gold Standard upon the successful certification under a given GS Approved Methodology. These may come in a number of forms.   Gold Standard recognises that typically the monitoring parameters included in GS-Approved Methodologies relate to Outcomes rather than Impacts. The use of the term Impact Statement reflects that these Outcomes may be used as a way of communicating the progress towards the impact sought and is typical of impact investment approaches."@en ,
                                                           "A aia:Claim regarding an aia:Agent aia:ImpactClaim, i.e. a verification claim"@en .


###  http://purl.org/aiaontology/gsvocabulary#Gold_Standard_Label
:Gold_Standard_Label rdf:type owl:Class ;
                     rdfs:subClassOf :Gold_Standard_Certified_Products ;
                     rdfs:comment "A Gold Standard Label is a type of Product that is Issued to a Project Developer but relates to the application of Gold Standard certification to a product issued by a third party. For example the application of Gold Standard Label to CERs."@en .


###  http://purl.org/aiaontology/gsvocabulary#GovernanceAndManagementSystem
:GovernanceAndManagementSystem rdf:type owl:Class ;
                               rdfs:subClassOf aia:Control ,
                                               aia:Procedure ;
                               rdfs:comment "Governance and Management System"@en ,
                                            "System of governance and management applied by a project (see Gold Standard for Sustainable Urban Development)."@en ;
                               skos:altLabel "GMS"@en .


###  http://purl.org/aiaontology/gsvocabulary#GreenhouseGas
:GreenhouseGas rdf:type owl:Class ;
               rdfs:subClassOf aia:Resource ;
               rdfs:comment "A gas that absorbs and emits radiation within the thermal infrared range. This process is the fundamental cause of the greenhouse effect. The primary greenhouse gases in Earth’s atmosphere are water vapor, carbon dioxide, methane, nitrous oxide, and ozone."@en ;
               rdfs:label "Greenhouse Gas"@en ;
               skos:altLabel "GHG"@en .


###  http://purl.org/aiaontology/gsvocabulary#HighConservationValue
:HighConservationValue rdf:type owl:Class ;
                       rdfs:subClassOf aia:Parameter .


###  http://purl.org/aiaontology/gsvocabulary#InterestedStakeholder
:InterestedStakeholder rdf:type owl:Class ;
                       rdfs:subClassOf :RelevantStakeholders ;
                       skos:definition "Any stakeholder who is interested (i.e. has expressed an interest) in the Project or its outcomes. They do not to be local or affected."@en .


###  http://purl.org/aiaontology/gsvocabulary#Issuance
:Issuance rdf:type owl:Class ;
          rdfs:subClassOf aia:Activity ;
          skos:definition "The issue by Gold Standard of a Gold Standard Certified Impact Statement or Product (such as a Gold Standard Verified Emissions Reduction (GS VER)). These are issued by Gold Standard following the successful completion of Performance Certification."@en .


###  http://purl.org/aiaontology/gsvocabulary#JustificationInformation
:JustificationInformation rdf:type owl:Class ;
                          rdfs:subClassOf aia:Claim ;
                          rdfs:comment "Along with an Output Indicator the information that must be provided to support the SDG Contributions claimed by a project. The information must credibly demonstrate how the Output Indicator can be used to show a positive influence on one or more SDG Indicators."@en ;
                          skos:related vcsv:Proof .


###  http://purl.org/aiaontology/gsvocabulary#KeyProjectInformation
:KeyProjectInformation rdf:type owl:Class ;
                       rdfs:subClassOf aia:Control ;
                       rdfs:comment "A template that captures high level project details in the early stages of development. The Key Project Information is used to support Eligibility Check."@en ;
                       rdfs:label "Key Project Information"@en ;
                       skos:altLabel "KPI"@en .


###  http://purl.org/aiaontology/gsvocabulary#Knowledge
:Knowledge rdf:type owl:Class ;
           rdfs:subClassOf aia:Resource ;
           rdfs:comment "The theoretical and/or practical understanding of a subject."@en .


###  http://purl.org/aiaontology/gsvocabulary#LandlockedLeastDevelopedCountry
:LandlockedLeastDevelopedCountry rdf:type owl:Class ;
                                 rdfs:subClassOf :LeastDevelopedCountry ;
                                 rdfs:label "Landlocked Least Developed Country"@en ;
                                 skos:altLabel "LLDC"@en .


###  http://purl.org/aiaontology/gsvocabulary#LeastDevelopedCountry
:LeastDevelopedCountry rdf:type owl:Class ;
                       rdfs:subClassOf aia:Location ;
                       rdfs:comment "The Least Developed Countries (LDCs) is a list of the countries that, according to the United Nations, exhibit the lowest indicators of socioeconomic development, with the lowest Human Development Index ratings of all countries in the world."@en ;
                       rdfs:label "Least Developed Country"@en ;
                       skos:altLabel "LDC"@en .


###  http://purl.org/aiaontology/gsvocabulary#Listed
:Listed rdf:type owl:Class ;
        rdfs:subClassOf aia:State ;
        rdfs:comment "Listed is a Certification status that an activity may achieve through successful completion of the Preliminary Review."@en ,
                     "TODO: should be a datatype & option for a datatype property, e.g. hasStatus?"@en .


###  http://purl.org/aiaontology/gsvocabulary#LocalStakeholder
:LocalStakeholder rdf:type owl:Class ;
                  rdfs:subClassOf :RelevantStakeholders ;
                  skos:definition "Stakeholders that reside or work within or in close proximity to the Project Area."@en .


###  http://purl.org/aiaontology/gsvocabulary#LowEmissionDevelopmentStrategies
:LowEmissionDevelopmentStrategies rdf:type owl:Class ;
                                  rdfs:subClassOf aia:Procedure ;
                                  rdfs:label "Low Emission Development Strategies"@en ;
                                  rdfs:seeAlso <http://ledsgp.org/?loclang=en_gb> ;
                                  skos:altLabel "LEDs"@en .


###  http://purl.org/aiaontology/gsvocabulary#MilleniumDevelopmentGoals
:MilleniumDevelopmentGoals rdf:type owl:Class ;
                           rdfs:subClassOf aia:Objective ;
                           rdfs:comment "The eight International Development goals adopted by the United Nations, 2000. The Millennium Development Goals conclude as of 2015 and are replaced by the Sustainable Development Goals."@en ;
                           rdfs:label "Millenium Development Goals"@en ;
                           skos:altLabel "MDGs"@en .


###  http://purl.org/aiaontology/gsvocabulary#MonitoringActivity
:MonitoringActivity rdf:type owl:Class ;
                    rdfs:subClassOf aia:Activity ;
                    rdfs:comment "The activity of monitoring a Project according its approved Monitoring Plan with the goal of quantifying the impact of a Project Activity"@en .


###  http://purl.org/aiaontology/gsvocabulary#MonitoringAndReportingPlan
:MonitoringAndReportingPlan rdf:type owl:Class ;
                            rdfs:subClassOf aia:Procedure ;
                            rdfs:comment "An initial plan and subsequent ongoing monitoring that is based on the systematic collection of data on specified indicators to provide indications of the extent to which outcomes are being achieved."@en .


###  http://purl.org/aiaontology/gsvocabulary#MonitoringPeriod
:MonitoringPeriod rdf:type owl:Class ;
                  rdfs:subClassOf aia:Period ;
                  rdfs:comment "The period of time for which a Monitoring Report covers and for which Verification and ultimately Certification is sought."@en .


###  http://purl.org/aiaontology/gsvocabulary#MonitoringReport
:MonitoringReport rdf:type owl:Class ;
                  rdfs:subClassOf aia:Claim ;
                  rdfs:comment "A report submitted by the Project Developer in support of Verification. The Monitoring Report includes reports against the parameters set in the Monitoring Plan plus any re-assessment, change or stakeholder feedback received during the Monitoring Period."@en .


###  http://purl.org/aiaontology/gsvocabulary#MonitoringReportingAndValidation
:MonitoringReportingAndValidation rdf:type owl:Class ;
                                  rdfs:subClassOf aia:Procedure ;
                                  rdfs:comment "System of collecting information, reporting and verifying that underpins Gold Standard for the Global Goals Principle 4 (Demonstration of Real Outcomes)"@en ;
                                  rdfs:label "Monitoring, Reporting, and Verification"@en ;
                                  skos:altLabel "MRV"@en .


###  http://purl.org/aiaontology/gsvocabulary#NationalAppropriateMitigationAction
:NationalAppropriateMitigationAction rdf:type owl:Class ;
                                     rdfs:subClassOf aia:Procedure ;
                                     rdfs:comment "NAMAs refer to any action that reduces emissions in developing countries and is prepared under the umbrella of a national governmental initiative. They can be policies directed at transformational change within an economic sector, or actions across sectors for a broader national focus. NAMAs are supported and enabled by technology, financing, and capacity-building and are aimed at achieving a reduction in emissions relative to ‘business as usual’ emissions in 2020."@en ;
                                     rdfs:label "National Appropriate Mitigation Action"@en ;
                                     rdfs:seeAlso <http://www4.unfccc.int/sites/nama/SitePages/Home.aspx> ;
                                     skos:altLabel "NAMA"@en .


###  http://purl.org/aiaontology/gsvocabulary#NationallyDeterminedContribution
:NationallyDeterminedContribution rdf:type owl:Class ;
                                  rdfs:subClassOf aia:Control ;
                                  rdfs:comment "According to Article 4 paragraph 2 of the Paris Agreement, each Party shall prepare, communicate and maintain successive nationally determined contributions (NDCs) that it intends to achieve. Parties shall pursue domestic mitigation measures, with the aim of achieving the objectives of such contributions."@en ;
                                  rdfs:label "Nationally Determined Contribution"@en ;
                                  skos:altLabel "NDC"@en .


###  http://purl.org/aiaontology/gsvocabulary#NonConformity
:NonConformity rdf:type owl:Class ;
               rdfs:subClassOf aia:Activity ;
               skos:definition "Non-conformity is a nonfulfillment, lapse in fulfilment or failure to meet a Requirement."@en .


###  http://purl.org/aiaontology/gsvocabulary#Observation
:Observation rdf:type owl:Class ;
             rdfs:subClassOf aia:Claim ;
             rdfs:comment "With an OBS, the Verification and Validation Body or The Gold Standard Secretariat provides an observation on possible future non-compliance with a requirement. Unlike Corrective Action Requests and Forward Action Requests, observations are suggestions or warnings and do not need necessarily to be formally corrected. They are given special attention during the next certification."@en ;
             skos:altLabel "OBS"@en .


###  http://purl.org/aiaontology/gsvocabulary#OngoingFinancialNeed
:OngoingFinancialNeed rdf:type owl:Class ;
                      rdfs:subClassOf aia:Procedure ;
                      rdfs:comment "Tool to demonstrate the ongoing need for financial support resulting from Gold Standard Certification and Issued Claims and Products. The approach is applied at 5 year Registration Renewal."@en ;
                      skos:altLabel "Ongoing Financial Need"@en .


###  http://purl.org/aiaontology/gsvocabulary#OnlinePlatform
:OnlinePlatform rdf:type owl:Class ;
                rdfs:subClassOf aia:Resource ;
                rdfs:comment "Gold Standard aspires to build an online user interface to support the use of GS4GG. The written version of the standard will underpin the online platform. During development and road-testing it is likely that an offline version will be used with the online platform commencing later."@en .


###  http://purl.org/aiaontology/gsvocabulary#OutputIndicator
:OutputIndicator rdf:type owl:Class ;
                 rdfs:subClassOf aia:Indicator ;
                 rdfs:comment "An indicator selected by the Project Developer, representing the tangible result of the Project. The indicator, along with the Justification Information and Quality Indicator and any Expert Stakeholder opinion is used to demonstrate SDG Contribution."@en .


###  http://purl.org/aiaontology/gsvocabulary#PerformanceReview
:PerformanceReview rdf:type owl:Class ;
                   rdfs:subClassOf <http://purl.org/aiaontology#Audit(n)> ;
                   rdfs:comment "A review conducted by Gold Standard, Technical Advisory Committe (TAC) and NGO Supporters on the Monitoring Report and Verification Opinion. The result of the Review may lead to Certification, Corrective Action Requests/Forward Action Requests/Observations being raised, or rejection."@en .


###  http://purl.org/aiaontology/gsvocabulary#PlannedEmissionsReduction
:PlannedEmissionsReduction rdf:type owl:Class ;
                           rdfs:subClassOf aia:Claim ;
                           rdfs:comment "A Planned Emission Reduction represents the expected (i.e., future) sequestration of 1 tonne of CO2e but does not represent an actual sequestration and accordingly shall not be used for carbon neutral claims until its conversion to a Verified Emission Reduction takes place."@en ;
                           rdfs:label "Planned Emissions Reduction"@en ;
                           skos:altLabel "PER"@en .


###  http://purl.org/aiaontology/gsvocabulary#PreliminaryReview
:PreliminaryReview rdf:type owl:Class ;
                   rdfs:subClassOf <http://purl.org/aiaontology#Audit(n)> ;
                   rdfs:comment "Review conducted once at the outset (i.e. at an early stage of project design and before Listing on the GS Registry) of a Project. Part of the Activity Cycle where Gold Standard assesses the Project Information in order to check whether an activity and approach is likely to be eligible for Gold Standard Certification. This procedure, if successful leads to Listed status. The requirements for the Project Design Documentation to be submitted at this stage are detailed in the latest version of GS4GG Principles & Requirements"@en .


###  http://purl.org/aiaontology/gsvocabulary#PreventativeAction
:PreventativeAction rdf:type owl:Class ;
                    rdfs:subClassOf aia:Activity ;
                    skos:definition "Action to prevent the occurrence of non-conformity(ies) or improve the effectiveness of its function."@en .


###  http://purl.org/aiaontology/gsvocabulary#ProductRequirements
:ProductRequirements rdf:type owl:Class ;
                     rdfs:subClassOf <http://purl.org/aiaontology#Control(n)> ;
                     rdfs:comment "The rules and requirements applicable to a particular Gold Standard Product, for example Verified Emissions Reductions."@en .


###  http://purl.org/aiaontology/gsvocabulary#ProgrammeOfActivities
:ProgrammeOfActivities rdf:type owl:Class ;
                       rdfs:subClassOf aia:Activity ;
                       rdfs:comment "FIX: characteristic: must have sub-activities; i.e. <program> containsCPA <project activity>+ inverse isActivityOf"@en ;
                       rdfs:label "Program of Activities"@en ;
                       skos:altLabel "PoA"@en ;
                       skos:definition "A programme is a linked series of Projects submitted to Gold Standard. A set of related activities with a common objective submitted to Gold Standard."@en .


###  http://purl.org/aiaontology/gsvocabulary#Project
:Project rdf:type owl:Class ;
         rdfs:subClassOf aia:Activity ;
         skos:definition "The activity or action being implemented for which Gold Standard Certification is sought."@en .


###  http://purl.org/aiaontology/gsvocabulary#ProjectActivity
:ProjectActivity rdf:type owl:Class ;
                 rdfs:subClassOf aia:Activity ;
                 rdfs:comment "An activity implemented additional to the Baseline Scenario (i.e. that would not have happened anyway) and with the express goal of achieving those results for which certification is sought."@en .


###  http://purl.org/aiaontology/gsvocabulary#ProjectArea
:ProjectArea rdf:type owl:Class ;
             rdfs:subClassOf aia:Location ;
             rdfs:comment "The Project Area is the physical spatial area or areas submitted for certification. It contains the area required to successfully manage the explicit objectives of the Project."@en .


###  http://purl.org/aiaontology/gsvocabulary#ProjectBoundary
:ProjectBoundary rdf:type owl:Class ;
                 rdfs:subClassOf aia:Location ;
                 rdfs:comment "The clearly defined physical boundary or edges of the project that delineate the Project Area from non-Project Areas."@en ;
                 skos:related cdmv:ProjectBoundary .


###  http://purl.org/aiaontology/gsvocabulary#ProjectCertificationRenewal
:ProjectCertificationRenewal rdf:type owl:Class ;
                             rdfs:subClassOf aia:Process ;
                             rdfs:comment "Project Certification Renewal is the process of re-certifying with Gold Standard every 5 years. This process follows the Project Design Certification process but specifically focuses on any changes to the Project Design Documentation and an updated Baseline Scenario and a demonstration of Ongoing Financial Need. Certain project types have adjusted renewal requirements, for example automatic renewal for a number of cycles or reduced/enhanced demonstration requirements. These are captured in the specific Activity Requirements."@en .


###  http://purl.org/aiaontology/gsvocabulary#ProjectDesignDocument
:ProjectDesignDocument rdf:type owl:Class ;
                       rdfs:subClassOf :ProjectDocumentation ;
                       rdfs:comment "Document that includes all information concerning project design and how it conforms to the Gold Standard Requirements."@en ;
                       rdfs:label "Project Design Document"@en ;
                       skos:altLabel "PDD"@en .


###  http://purl.org/aiaontology/gsvocabulary#ProjectDeveloper
:ProjectDeveloper rdf:type owl:Class ;
                  rdfs:subClassOf aia:Role ;
                  rdfs:comment "FIX: are these Roles or subclasses of Agent"@en ,
                               """The person or entity that holds or is applying for certification and therefore responsible for demonstrating compliance with the requirements upon which Gold Standard certification is based.  The Project Developer shall be one individual or entity only.
The developer and/or manager of the project."""@en .


###  http://purl.org/aiaontology/gsvocabulary#ProjectDocumentation
:ProjectDocumentation rdf:type owl:Class ;
                      rdfs:subClassOf aia:Claim ;
                      rdfs:comment "Umbrella term for all project design and monitoring documentation that demonstrates in detail how the Requirements are met. This can include Gold Standard Templates such as Project Design Documents and Monitoring Reports as well as Supporting Documents such as charts, maps or spreadsheets."@en ;
                      skos:related vcsv:Proof .


###  http://purl.org/aiaontology/gsvocabulary#ProjectParticipant
:ProjectParticipant rdf:type owl:Class ;
                    rdfs:subClassOf aia:Role ;
                    rdfs:comment """A Project Participant is an individual or entity that is contributing to the generation of the certified impacts.

Any party or individual who is working closely with the Client to carry out the activities or who has provided written approval for a project. Activity participants shall be collectively represented by the Client or his Representative."""@en .


###  http://purl.org/aiaontology/gsvocabulary#ProjectRepresentative
:ProjectRepresentative rdf:type owl:Class ;
                       rdfs:subClassOf aia:Role ;
                       rdfs:comment "Refers to the person or entity that will serve as the focal point for the project. This representative will have sole or joint authority to communicate with the Gold Standard Secretariat regarding all matters related to a project’s certification, alteration or expansion. The project representative can be more than one individual or entity."@en .


###  http://purl.org/aiaontology/gsvocabulary#ProjectScenario
:ProjectScenario rdf:type owl:Class ;
                 rdfs:subClassOf aia:State ;
                 rdfs:comment "The Project Scenario is defined as the scenario that will exist once the Project is implemented and operational."@en .


###  http://purl.org/aiaontology/gsvocabulary#QualityIndicator
:QualityIndicator rdf:type owl:Class ;
                  rdfs:subClassOf aia:Indicator ;
                  rdfs:comment "Information that is submitted with the Output Indicator and Justification Information that together can be used to demonstrate an SDG Contribution. The Quality Indicator is specifically used in to build upon the Output Indicator which quantifies the results by adding information on the quality of the result."@en .


###  http://purl.org/aiaontology/gsvocabulary#RelevantStakeholders
:RelevantStakeholders rdf:type owl:Class ;
                      rdfs:subClassOf aia:Agent ;
                      rdfs:comment """TODO: generic property like fulfillsRoleRequirement
Can refine later if needed, e.g. elaborate on what requirements there are to fulfill the requirement to be an stakeholder etc."""@en ;
                      skos:definition "The collective term for local, affected, interested and expert stakeholders."@en .


###  http://purl.org/aiaontology/gsvocabulary#RenewableEnergy
:RenewableEnergy rdf:type owl:Class ;
                 rdfs:subClassOf aia:Activity ;
                 rdfs:comment "The generation of energy from clean, sustainable, renewable processes."@en ;
                 skos:altLabel "RE"@en .


###  http://purl.org/aiaontology/gsvocabulary#RenewableEnergyCertificate
:RenewableEnergyCertificate rdf:type owl:Class ;
                            rdfs:subClassOf aia:Claim ,
                                            :Certification ;
                            rdfs:comment "Renewable Energy Certificates are tradable, non-tangible energy commodities that represent proof that 1 megawatt-hour (MWh) of electricity was generated from an eligible renewable energy resource (renewable electricity) and was fed into the shared system of power lines which transport energy. Renewable Energy Certificates provide a mechanism for the purchase of renewable energy that is added to and pulled from the electrical grid."@en ;
                            rdfs:label "Renewable Energy Certificate"@en ;
                            skos:altLabel "REC"@en .


###  http://purl.org/aiaontology/gsvocabulary#Requirements
:Requirements rdf:type owl:Class ;
              rdfs:comment "Elements (rules, procedures, guidelines) that the activity must conform to in order to proceed through Validation/Verification and ultimately Certification."@en .


###  http://purl.org/aiaontology/gsvocabulary#Risk
:Risk rdf:type owl:Class ;
      rdfs:subClassOf aia:Parameter ;
      rdfs:comment "Actions taken to lessen the probability or negative consequences, or both, associated with a risk."@en .


###  http://purl.org/aiaontology/gsvocabulary#SDGImpact
:SDGImpact rdf:type owl:Class ;
           rdfs:subClassOf aia:Output ;
           rdfs:comment "A direct, positive contribution to a Sustainable Development Goal generated by a Project."@en .


###  http://purl.org/aiaontology/gsvocabulary#Scale
:Scale rdf:type owl:Class ;
       rdfs:comment "The Scale of a project may refer to a variety of definitions for example areal extent, size of impact or units provided. Scale is not limited in Gold Standard for the Global Goals but is dealt with in the Activity Requirements, Methodologies and Product Requirements where specific definitions and requirements are included."@en .


###  http://purl.org/aiaontology/gsvocabulary#Shapefile
:Shapefile rdf:type owl:Class ;
           rdfs:comment "A shapefile is a digital vector (non-topological) storage format for storing geometric location and associated attribute information. A shapefile can consist of points, lines or polygons."@en ;
           skos:related aia:Location .


###  http://purl.org/aiaontology/gsvocabulary#StakeholderConsultation
:StakeholderConsultation rdf:type owl:Class ;
                         rdfs:subClassOf aia:Activity ;
                         rdfs:label "Stakeholder Consultation"@en ;
                         rdfs:seeAlso <https://www.ofenmacher.org/files/1914/2331/2357/The-Gold-Standard-Principles-FINAL-270513.pdf> ;
                         skos:definition "The process and requirements associated with carrying out stakeholder consultation as part of Principle 3, Stakeholder Inclusivity."@en .


###  http://purl.org/aiaontology/gsvocabulary#StakeholderFeedbackRound
:StakeholderFeedbackRound rdf:type owl:Class ;
                          rdfs:subClassOf <http://purl.org/aiaontology#Control(n)> ;
                          rdfs:comment "An opportunity for Relevant Stakeholders to provide feedback about a project as part of the process towards fulfilling Principle 3 – Stakeholder Inclusivity."@en ,
                                       "Losweg: die geleentheid om StakeholderConsultation uit te voer"@en ;
                          rdfs:label "Stakeholder Feedback Round"@en .


###  http://purl.org/aiaontology/gsvocabulary#ValidationAndVerificationBody
:ValidationAndVerificationBody rdf:type owl:Class ;
                               rdfs:subClassOf aia:LegalPerson ;
                               rdfs:label "(Gold Standard) Validation and Verification Body"@en ;
                               skos:altLabel "VVB"@en ;
                               skos:definition "A Gold Standard approved audit organisation appointed by and on behalf of the Project Developer to carry out an audit and assessment in order to provide a Validation or Verification Report to Gold Standard in order to ultimately support Certification or rejection."@en .


#################################################################
#    Individuals
#################################################################

###  http://purl.org/aiaontology/gsvocabulary#AmericanNationalStandardsInstitute
:AmericanNationalStandardsInstitute rdf:type owl:NamedIndividual ,
                                             aia:LegalPerson ;
                                    rdfs:comment "American National Standards Institute"@en ;
                                    rdfs:seeAlso <https://www.ansica.org> ;
                                    skos:altLabel "ANSI"@en .


###  http://purl.org/aiaontology/gsvocabulary#AvertedDisabilityAdjustedLifeYear
:AvertedDisabilityAdjustedLifeYear rdf:type owl:NamedIndividual ,
                                            aia:Parameter ;
                                   rdfs:comment "A measure of mortality and morbidity used to demonstrate project impact on SDG 3.  The quantification and certification of ADALYs is undertaken via the use of a GS-Methodology."@en ;
                                   skos:altLabel "ADALY"@en .


###  http://purl.org/aiaontology/gsvocabulary#CDMExecutiveBoard
:CDMExecutiveBoard rdf:type owl:NamedIndividual ,
                            aia:LegalPerson ;
                   rdfs:comment "Executive Board of the Clean Development Mechanism."@en .


###  http://purl.org/aiaontology/gsvocabulary#EuropeanUnion
:EuropeanUnion rdf:type owl:NamedIndividual ,
                        aia:LegalPerson .


###  http://purl.org/aiaontology/gsvocabulary#GoldStandardFoundation
:GoldStandardFoundation rdf:type owl:NamedIndividual ,
                                 aia:LegalPerson ;
                        rdfs:comment "The owner and operator of Gold Standard for the Global Goals. Gold Standard is a Swiss-based non-profit whose Vision focuses on Climate Security and Sustainable Development for all."@en ;
                        rdfs:seeAlso <https://www.goldstandard.org> .


###  http://purl.org/aiaontology/gsvocabulary#GoldStandardTechnicalAdvisoryCommittee
:GoldStandardTechnicalAdvisoryCommittee rdf:type owl:NamedIndividual ,
                                                 aia:LegalPerson ;
                                        rdfs:comment "The Gold Standard Technical Advisory Committee (GS TAC) is responsible for ensuring the rigor and integrity in all our work, proven existing programs and innovative new initiatives. The TAC is an independent body composed of market specialists that provide expertise, guidance and decisions."@en .


###  http://purl.org/aiaontology/gsvocabulary#HighConservationValue
:HighConservationValue rdf:type owl:NamedIndividual ,
                                aia:Parameter .


###  http://purl.org/aiaontology/gsvocabulary#InternationalSocialAndEnvironmentalAccreditationAndLabeling
:InternationalSocialAndEnvironmentalAccreditationAndLabeling rdf:type owl:NamedIndividual ,
                                                                      aia:LegalPerson ;
                                                             rdfs:seeAlso <https://www.isealalliance.org/> .


###  http://purl.org/aiaontology/gsvocabulary#InternationalStandardsOrganisation
:InternationalStandardsOrganisation rdf:type owl:NamedIndividual ,
                                             aia:LegalPerson ;
                                    rdfs:label "International Standards Organisation"@en ;
                                    rdfs:seeAlso <http://purl.org/aiaontology/www.iso.org> ;
                                    skos:altLabel "ISO"@en .


###  http://purl.org/aiaontology/gsvocabulary#InternationalUnionForTheConservationOfNature
:InternationalUnionForTheConservationOfNature rdf:type owl:NamedIndividual ,
                                                       aia:LegalPerson ;
                                              rdfs:comment "International Union for the Conservation of Nature"@en ;
                                              rdfs:seeAlso <http://purl.org/aiaontology/www.iucn.org> ;
                                              skos:altLabel "IUCN"@en .


###  http://purl.org/aiaontology/gsvocabulary#NationalDevelopmentStrategy
:NationalDevelopmentStrategy rdf:type owl:NamedIndividual ,
                                      aia:Procedure ;
                             rdfs:comment "National Development Strategy"@en ;
                             rdfs:seeAlso <http://www.un.org/en/development/desa/policynotes.html> ;
                             skos:altLabel "NDS"@en .


###  http://purl.org/aiaontology/gsvocabulary#ParisAgreement
:ParisAgreement rdf:type owl:NamedIndividual ,
                         aia:Control ;
                rdfs:comment "The Paris Agreement, or Paris climate accord and Paris climate agreement, is an agreement within the United Nations Framework Convention on Climate Change (UNFCCC) dealing with greenhouse gas emissions mitigation, adaptation and finance starting in the year 2020."@en .


###  http://purl.org/aiaontology/gsvocabulary#RoundtableForSustainablePalmOil
:RoundtableForSustainablePalmOil rdf:type owl:NamedIndividual ,
                                          aia:LegalPerson ;
                                 rdfs:comment "Roundtable for Sustainable Palm Oil"@en ;
                                 rdfs:seeAlso "https://www.rspo.org"@en ;
                                 skos:altLabel "RSPO"@en .


#################################################################
#    Annotations
#################################################################

:HighConservationValue rdfs:comment "A biological, ecological, social or cultural value of outstanding significance or critical importance."@en ;
                       skos:altLabel "HCV"@en .


###  Generated by the OWL API (version 4.5.9.2019-02-01T07:24:44Z) https://github.com/owlcs/owlapi
